

作业1: 求 $\lambda E - A$

$$A = \begin{pmatrix} 4 & 6 & 0 \\ -3 & -5 & 0 \\ 3 & -6 & 1 \end{pmatrix} \Rightarrow \lambda E - A = \begin{pmatrix} \lambda-4 & -6 & 0 \\ 3 & \lambda+5 & 0 \\ 3 & 6 & \lambda-1 \end{pmatrix}$$

$$\because \lambda_1 = 3, \lambda_2 = -6 \text{ 常数} \Rightarrow \therefore D_1(\lambda) = 1$$

$$D_3(\lambda) = \det(\lambda E - A) = \begin{vmatrix} \lambda-4 & -6 & 0 \\ 3 & \lambda+5 & 0 \\ 3 & 6 & \lambda-1 \end{vmatrix} = (\lambda-1) \cdot \begin{vmatrix} \lambda-4 & -6 \\ 3 & \lambda+5 \end{vmatrix} \\ = (\lambda-1)^2 (\lambda+2)$$

$$D_2(\lambda) \text{ 10m33} = \begin{vmatrix} \lambda-4 & -6 \\ 3 & \lambda+5 \end{vmatrix} = (\lambda+2)(\lambda-1) \Rightarrow D_2(\lambda) = (\lambda-1)$$

$$2^\circ m_{\lambda 3} = \begin{vmatrix} 3 & \lambda+5 \\ 3 & 6 \end{vmatrix} = -3(\lambda-1)$$

$$\therefore d_k(\lambda) = D_k(\lambda) / D_{k-1}(\lambda) \Rightarrow \text{Smith} \begin{pmatrix} 1 & 0 & 0 \\ 0 & \lambda-1 & 0 \\ 0 & 0 & (\lambda-1)(\lambda+2) \end{pmatrix} \\ \Rightarrow d_1^k = 1 \quad d_2(\lambda) = (\lambda-1)(\lambda+2) \\ d_3(\lambda) = \lambda-1$$

$$\text{作业2: } A(\lambda) = \begin{bmatrix} 1-\lambda & \lambda^2 & \lambda \\ \lambda & \lambda & -\lambda \\ 1+\lambda^2 & \lambda^2 & \lambda \end{bmatrix} \xrightarrow{r_3-r_1} \begin{bmatrix} 1-\lambda & \lambda^2 & \lambda \\ \lambda & \lambda & -\lambda \\ \lambda^2+\lambda & 0 & 0 \end{bmatrix}$$

$$\xrightarrow{r_2+r_1, r_1 \leftrightarrow r_2} \begin{bmatrix} 1-\lambda & \lambda^2 & \lambda \\ 1 & \lambda(\lambda+1) & 0 \\ \lambda(\lambda+1) & 0 & 0 \end{bmatrix} \xrightarrow{r_2 - (1+\lambda)r_1} \begin{bmatrix} 1 & \lambda(\lambda+1) & 0 \\ 0 & \lambda^3 + \lambda^2 - \lambda & \lambda \\ \lambda(\lambda+1) & 0 & 0 \end{bmatrix}$$

$$\xrightarrow{r_3 - \lambda(\lambda+1)r_1} \begin{bmatrix} 1 & \lambda(\lambda+1) & 0 \\ 0 & \lambda^3 + \lambda^2 - \lambda & \lambda \\ 0 & -\lambda^2(\lambda+1)^2 & 0 \end{bmatrix} \xrightarrow{(2 - \lambda(\lambda+1))c_1} \begin{bmatrix} 1 & 0 & 0 \\ 0 & \lambda^3 + \lambda^2 - \lambda & \lambda \\ 0 & -\lambda^2(\lambda+1)^2 & 0 \end{bmatrix}$$

$$\xrightarrow{(2 \leftrightarrow 3)} \begin{bmatrix} 1 & 0 & 0 \\ 0 & \lambda & 0 \\ 0 & 0 & -\lambda^2(\lambda+1)^2 \end{bmatrix}$$

$$\Rightarrow d_1(\lambda) = 1$$

$$d_2(\lambda) = \lambda$$

$$d_3(\lambda) = \lambda^2(\lambda+1)^2 \text{ 整除}$$

$$\Rightarrow \text{Smith} \begin{bmatrix} 1 & 0 & 0 \\ 0 & \lambda & 0 \\ 0 & 0 & \lambda^2(\lambda+1)^2 \end{bmatrix}$$

deli得力

Date: 1

3. $A(\lambda) = \begin{bmatrix} -\lambda(\lambda+1) & 0 & 0 \\ 0 & \lambda & 0 \\ 0 & 0 & (\lambda+1)^2 \end{bmatrix}$ 则初等因子为 $\{\lambda, \lambda, \lambda+1, (\lambda+1)^2\}$

从 $d_3(\lambda)$ 开始, $d_3(\lambda) = \lambda(\lambda+1)^2$

$d_2(\lambda) = \lambda(\lambda+1)$

$d_1(\lambda) = 1$

则 Smith: $\begin{bmatrix} 1 & 0 & 0 \\ 0 & \lambda(\lambda+1) & 0 \\ 0 & 0 & \lambda(\lambda+1)^2 \end{bmatrix}$

4. 初等因子共 $n=7$ 阶, 待求 $d_i(\lambda) \rightarrow d_7(\lambda)$

初等因子: $1^\circ \lambda^2, \lambda, \lambda$

$2^\circ (\lambda-1)^2$

$3^\circ (\lambda+1)$

$\Rightarrow d_7(\lambda) = \lambda^2(\lambda-1)^2(\lambda+1)$ $d_6(\lambda) = \lambda$ $d_5 = \lambda$

$d_4 = 1 = d_3 = d_2 = d_1$

\Rightarrow 不变因子 $1, 1, 1, 1, \lambda, \lambda, \lambda^2(\lambda-1)^2(\lambda+1)$

Smith:

diag: $(1, 1, 1, 1, \lambda, \lambda, \lambda^2(\lambda-1)^2(\lambda+1))$